Move some trace-related defs into TraceUtil

raft/OutputImpliesAppliedInterface.v
@@ -4,9 +4,10 @@ Require Import Arith.
 Require Import Net.
 Require Import Util.
 Require Import VerdiTactics.
-Require Import Raft.
 
+Require Import Raft.
 Require Import CommonDefinitions.
+Require Import TraceUtil.
 
 Section OutputImpliesApplied.
   Context {orig_base_params : BaseParams}.
@@ -18,33 +19,6 @@ Section OutputImpliesApplied.
 
   Variables client id : nat.
 
-  Definition in_output_list (os : list raft_output) :=
-    exists o,
-      In (ClientResponse client id o) os.
-
-  Definition is_client_response (out : raft_output) : bool :=
-    match out with
-      | ClientResponse c i _ => andb (beq_nat client c) (beq_nat id i)
-      | NotLeader _ _ => false
-    end.
-
-  Definition in_output_list_dec (os : list raft_output) :
-    {in_output_list os} + {~ in_output_list os}.
-  Proof.
-    unfold in_output_list.
-    destruct (find is_client_response os) eqn:?.
-    - find_apply_lem_hyp find_some. break_and.
-      unfold is_client_response in *. break_match; try discriminate.
-      subst. do_bool. break_and. do_bool. subst. left. eauto.
-    - right. intro. break_exists.
-      eapply find_none in H; eauto. unfold is_client_response in *.
-      find_apply_lem_hyp Bool.andb_false_elim. intuition; do_bool; congruence.
-  Qed.
-
-  Definition in_output (tr : list (name * (raft_input + list raft_output))) : Prop :=
-    exists os h,
-      In (h, inr os) tr /\
-      in_output_list os.
 
   Definition in_applied_entries (net : network) : Prop :=
     exists e,
@@ -59,7 +33,7 @@ Section OutputImpliesApplied.
       output_implies_applied :
         forall client id failed net tr,
           step_f_star step_f_init (failed, net) tr ->
-          in_output client id tr ->
+          key_in_output_trace client id tr ->
           in_applied_entries client id net
     }.
 End OutputImpliesApplied.
