raft/AppliedImpliesInputInterface.v
@@ -1,20 +1,14 @@
 Require Import List.
 Require Import Net.
+
 Require Import Raft.
 Require Import CommonDefinitions.
+Require Import TraceUtil.
 
 Section AppliedImpliesInputInterface.
   Context {orig_base_params : BaseParams}.
   Context {one_node_params : OneNodeParams orig_base_params}.
   Context {raft_params : RaftParams orig_base_params}.
-
-  Section inner.
-    Variables client id : nat.
-
-    Definition in_input (tr : list (name * (raft_input + list raft_output))) : Prop :=
-      exists h i,
-        In (h, inl (ClientRequest client id i)) tr.
-  End inner.
 
   Class applied_implies_input_interface : Prop :=
     {
@@ -24,6 +18,6 @@ Section AppliedImpliesInputInterface.
           eClient e = client ->
           eId e = id ->
           In e (applied_entries (nwState net)) ->
-          in_input client id tr
+          key_in_input_trace client id tr
     }.
 End AppliedImpliesInputInterface.
