raft/TraceUtil.v
@@ -1,0 +1,62 @@
+Require Import List.
+Import ListNotations.
+Require Import Arith.
+
+Require Import Net.
+Require Import VerdiTactics.
+Require Import Util.
+Require Import Raft.
+
+Section TraceUtil.
+  Context {orig_base_params : BaseParams}.
+  Context {one_node_params : OneNodeParams orig_base_params}.
+  Context {raft_params : RaftParams orig_base_params}.
+
+  Definition key_in_output_list (client id : nat) (os : list raft_output) :=
+    exists o,
+      In (ClientResponse client id o) os.
+
+  Definition is_client_response_with_key (client id : nat) (out : raft_output) : bool :=
+    match out with
+      | ClientResponse c i _ => andb (beq_nat client c) (beq_nat id i)
+      | NotLeader _ _ => false
+    end.
+
+  Definition key_in_output_list_dec (client id : nat) (os : list raft_output) :
+    {key_in_output_list client id os} + {~ key_in_output_list client id os}.
+  Proof.
+    unfold key_in_output_list.
+    destruct (find (is_client_response_with_key client id) os) eqn:?.
+    - find_apply_lem_hyp find_some. break_and.
+      unfold is_client_response_with_key in *. break_match; try discriminate.
+      subst. do_bool. break_and. do_bool. subst. left. eauto.
+    - right. intro. break_exists.
+      eapply find_none in H; eauto. unfold is_client_response_with_key in *.
+      find_apply_lem_hyp Bool.andb_false_elim. intuition; do_bool; congruence.
+  Qed.
+
+  Definition key_in_output_trace (client id : nat)
+             (tr : list (name * (raft_input + list raft_output))) : Prop :=
+    exists os h,
+      In (h, inr os) tr /\
+      key_in_output_list client id os.
+
+  Definition key_in_input_trace (client id : nat)
+             (tr : list (name * (raft_input + list raft_output))) : Prop :=
+      exists h i,
+        In (h, inl (ClientRequest client id i)) tr.
+  
+  Definition is_output_with_key (client id : nat)
+             (trace_entry : (name * (raft_input + list raft_output))) :=
+    match trace_entry with
+      | (_, inr os) => if key_in_output_list_dec client id os then true else false
+      | _ => false
+    end.
+
+  Definition is_input_with_key (client id: nat)
+             (trace_entry : (name * (raft_input + list raft_output))) :=
+    match trace_entry with
+      | (_, inl (ClientRequest c i _)) => andb (beq_nat client c) (beq_nat id i)
+      | _ => false
+    end.
+End TraceUtil.
